split Sequences into multiple modules

SeqOfSeq.dfy
@@ -19,4 +19,132 @@ module SeqOfSeq {
     if |a| == 0 then [] else concat_seq(drop_last(a)) + last(a)
   }
 
+    /* concatenating two sequences of sequences is equivalent to concatenating
+  each sequence of sequences seperately, and then concatenating the two resulting 
+  sequences together */
+  lemma lemma_seq_concat_adds<T>(A:seq<seq<T>>, B:seq<seq<T>>)
+    ensures seq_concat(A + B) == seq_concat(A) + seq_concat(B)
+  {
+    if |A| == 0 {
+      assert A+B == B;
+    } else {
+      calc == {
+        seq_concat(A + B);
+          { assert (A + B)[0] == A[0];  assert (A + B)[1..] == A[1..] + B; }
+        A[0] + seq_concat(A[1..] + B);
+        A[0] + seq_concat(A[1..]) + seq_concat(B);
+        seq_concat(A) + seq_concat(B);
+      }
+    }
+  }
+
+  // proves sequence addition
+  lemma lemma_concat_seq_addition<A>(a: seq<seq<A>>, b: seq<seq<A>>)
+  ensures concat_seq(a + b) == concat_seq(a) + concat_seq(b)
+  {
+    if b == [] {
+      calc {
+        concat_seq(a + b);
+        { assert a + b == a; }
+        concat_seq(a);
+        {
+          reveal_concat_seq();
+          assert concat_seq(b) == [];
+        }
+        concat_seq(a) + concat_seq(b);
+      }
+    } else {
+      calc {
+        concat_seq(a + b);
+        { reveal_concat_seq(); }
+        concat_seq(drop_last(a + b)) + last(a + b);
+        {
+          assert drop_last(a + b) == a + drop_last(b);
+          assert last(a + b) == last(b);
+        }
+        concat_seq(a + drop_last(b)) + last(b);
+        {
+          lemma_concat_seq_addition(a, drop_last(b));
+        }
+        concat_seq(a) + concat_seq(drop_last(b)) + last(b);
+        { reveal_concat_seq(); }
+        concat_seq(a) + concat_seq(b);
+      }
+    }
+  }
+
+  /* concatenates the sequence of sequences into a single sequence. 
+  works by adding elements from last to first */
+  function method seq_concat_reverse<T>(seqs: seq<seq<T>>): seq<T>
+  decreases |seqs|
+  {
+    if |seqs| == 0 then []
+    else seq_concat_reverse(drop_last(seqs)) + last(seqs)
+  }
+
+  /* concatenating two reversed sequences of sequences is the same as reversing two 
+  sequences of sequences and then adding the two resulting sequences together */
+  lemma lemma_seq_concat_reverse_adds<T>(A:seq<seq<T>>, B:seq<seq<T>>)
+  ensures seq_concat_reverse(A + B) == seq_concat_reverse(A) + seq_concat_reverse(B)
+  {
+    if |B| == 0 {
+      assert seq_concat_reverse(B) == [];
+      assert A+B == A;
+    } else {
+      calc == {
+        seq_concat_reverse(A + B);
+          { assert last(A + B) == last(B);  assert drop_last(A + B) == A + drop_last(B); }
+        seq_concat_reverse(A + drop_last(B)) + last(B);
+        seq_concat_reverse(A) + seq_concat_reverse(drop_last(B)) + last(B);
+        seq_concat_reverse(A) + seq_concat_reverse(B);
+      }
+    }
+  }
+
+  /* both methods of concatenating sequence (starting from front v. starting from back)
+  result in the same sequence */
+  lemma lemma_seq_concat_and_seq_concat_reverse_are_equivalent<T>(seqs: seq<seq<T>>)
+    ensures seq_concat(seqs) == seq_concat_reverse(seqs)
+  {
+    if |seqs| == 0 {
+    } else {
+      calc == {
+        seq_concat_reverse(seqs);
+        seq_concat_reverse(drop_last(seqs)) + last(seqs);
+          { lemma_seq_concat_and_seq_concat_reverse_are_equivalent(drop_last(seqs)); }
+        seq_concat(drop_last(seqs)) + last(seqs);
+        seq_concat(drop_last(seqs)) + seq_concat([last(seqs)]);
+          { lemma_seq_concat_adds(drop_last(seqs), [last(seqs)]); 
+        assert seqs == drop_last(seqs) + [last(seqs)]; }
+        seq_concat(seqs);
+      }
+    }
+  }
+
+  /* the concatenated sequence's length is greater than or equal to 
+  each individual inner sequence's length */
+  lemma lemma_concat_seq_length_ge_single_element_length<A>(a: seq<seq<A>>, i: int)
+  requires 0 <= i < |a|
+  ensures |concat_seq(a)| >= |a[i]|
+  {
+    reveal_concat_seq();
+    if i < |a| - 1 {
+      lemma_concat_seq_length_ge_single_element_length(a[..|a|-1], i);
+    }
+  }
+
+  /* the length of concatenating sequence in a sequence together will be no longer 
+  than the length of the original sequence of sequences multiplied by the length of 
+  the longest sequence */
+  lemma lemma_concat_seq_length_le_mul<A>(a: seq<seq<A>>, t: int)
+  requires forall i | 0 <= i < |a| :: |a[i]| <= t
+  ensures |concat_seq(a)| <= |a| * t
+  {
+    reveal_concat_seq();
+    if |a| == 0 {
+    } else {
+      lemma_concat_seq_length_le_mul(a[..|a|-1], t);
+    }
+  }
+
 }
