SeqHigherLevel.dfy
@@ -1,0 +1,35 @@
+module SeqHigherLevel { 
+  // applies a transformation function on the sequence
+  function method {:opaque} Map<E,R>(f: (E ~> R), s: seq<E>): (result: seq<R>)
+    requires forall i :: 0 <= i < |s| ==> f.requires(s[i])
+    ensures |result| == |s|
+    ensures forall i :: 0 <= i < |s| ==> result[i] == f(s[i]);
+    reads set i, o | 0 <= i < |s| && o in f.reads(s[i]):: o
+  {
+    if |s| == 0 then []
+    else  [f(s[0])] + Map(f, s[1..])
+  }
+
+  // uses a selection function to select elements from the sequence
+  function method {:opaque} filter<E>(f : (E ~> bool), s: seq<E>): (result: seq<E>)
+    requires forall i :: 0 <= i < |s| ==> f.requires(s[i])
+    ensures |result| <= |s|
+    ensures forall i: nat :: i < |result| && f.requires(result[i]) ==> f(result[i])
+    reads f.reads
+  {
+    if |s| == 0 then []
+    else ((if f(s[0]) then [s[0]] else []) + filter(f, s[1..]))
+  }
+  
+  function method {:opaque} fold_left<A,E>(f: (A, E) -> A, init: A, s: seq<E>): A
+  {
+    if |s| == 0 then init
+    else fold_left(f, f(init, s[0]), s[1..])
+  }
+
+  function method {:opaque} fold_right<A,E>(f: (A, E) -> A, init: A, s: seq<E>): A
+  {
+    if |s| == 0 then init
+    else f(fold_right(f, init, s[1..]), s[0])
+  }
+}
