Sequences.dfy
@@ -8,7 +8,7 @@ module Seq {
   import opened Options
   import Math = Mathematics
   import opened SeqLast
-  
+
   /* a sequence that is sliced at the jth element concatenated with that same
   sequence sliced from the jth element is equal to the original, unsliced sequence */
   lemma lemma_split_act<T>(intseq: seq<T>, j: int)
@@ -134,40 +134,6 @@ module Seq {
       Some(index_of(s, v))
     else
       None
-  }
-
-  // applies a transformation function on the sequence
-  function method {:opaque} Map<E,R>(f: (E ~> R), s: seq<E>): (result: seq<R>)
-    requires forall i :: 0 <= i < |s| ==> f.requires(s[i])
-    ensures |result| == |s|
-    ensures forall i :: 0 <= i < |s| ==> result[i] == f(s[i]);
-    reads set i, o | 0 <= i < |s| && o in f.reads(s[i]):: o
-  {
-    if |s| == 0 then []
-    else  [f(s[0])] + Map(f, s[1..])
-  }
-
-  // uses a selection function to select elements from the sequence
-  function method {:opaque} filter<E>(f : (E ~> bool), s: seq<E>): (result: seq<E>)
-    requires forall i :: 0 <= i < |s| ==> f.requires(s[i])
-    ensures |result| <= |s|
-    ensures forall i: nat :: i < |result| && f.requires(result[i]) ==> f(result[i])
-    reads f.reads
-  {
-    if |s| == 0 then []
-    else ((if f(s[0]) then [s[0]] else []) + filter(f, s[1..]))
-  }
-  
-  function method {:opaque} fold_left<A,E>(f: (A, E) -> A, init: A, s: seq<E>): A
-  {
-    if |s| == 0 then init
-    else fold_left(f, f(init, s[0]), s[1..])
-  }
-
-  function method {:opaque} fold_right<A,E>(f: (A, E) -> A, init: A, s: seq<E>): A
-  {
-    if |s| == 0 then init
-    else f(fold_right(f, init, s[1..]), s[0])
   }
 
   // slices out a specific position's value from the sequence and returns the new sequence
